

M378K: November 3rd, 2025.

More on Estimators.

Def'n. The **bias** of an estimator $\hat{\theta}$ for θ is

$$\text{bias}(\hat{\theta}) = \mathbb{E}[\hat{\theta}] - \theta$$

If $\boxed{\text{bias}(\hat{\theta}) = 0}$, we say that $\hat{\theta}$ is **unbiased** for θ .

Def'n. The **mean squared error** of $\hat{\theta}$ is

$$\begin{aligned} \text{MSE}(\hat{\theta}) &= \text{Var}(\hat{\theta}) + (\text{bias}(\hat{\theta}))^2 \\ &= \mathbb{E}[(\hat{\theta} - \theta)^2] \end{aligned}$$

Def'n. An estimator $\hat{\theta}$ is **uniformly minimum variance unbiased estimator (UMVUE)**

of θ if: $\left\{ \begin{array}{l} \bullet \hat{\theta} \text{ is unbiased} \\ \bullet \text{MSE}(\hat{\theta}) \leq \text{MSE}(\hat{\theta}') \text{ for all other unbiased estimators } \hat{\theta}' \text{ of } \theta. \end{array} \right.$

Example. These are **UMVUE**:

- \bar{Y} for μ where (Y_1, \dots, Y_n) is a random sample from $N(\mu, \sigma_0)$
- \bar{Y} for p where (Y_1, \dots, Y_n) is a random sample from $B(p)$

$$s^2 = \frac{1}{n-1} \sum_{i=1}^n (Y_i - \bar{Y})^2$$

for σ^2 where (Y_1, \dots, Y_n) is a random sample from $N(\mu, \sigma)$ w/ **both** parameters unknown

Def'n. An estimator $\hat{\theta}$ is said to be **linear** if it's of the form

$$\hat{\theta} = \alpha_1 Y_1 + \alpha_2 Y_2 + \dots + \alpha_n Y_n$$

where α_i are all constants

e.g., \bar{Y}

Problem 15.3. Let Y_1, Y_2, \dots, Y_n be a random sample from a continuous distribution with probability density function

$$f_Y(y) = \frac{\alpha y^{\alpha-1}}{\theta^\alpha} \mathbf{1}_{[0, \theta]}(y)$$

with a known parameter $\alpha > 0$ and an unknown parameter $\theta > 0$. We propose the estimator $\hat{\theta} = \max(Y_1, \dots, Y_n)$. Is this estimator unbiased? If not, how would you modify it to create an unbiased estimator? What is the mean-squared error of the unbiased estimator you obtained?

→: $\hat{\theta} = Y_{(n)} = \max(Y_1, \dots, Y_n)$

$E[\hat{\theta}] = E[Y_{(n)}] = ?$

$g_{(n)}(y) = n \cdot (F_Y(y))^{n-1} \cdot f_Y(y)$

$E[Y_{(n)}] = \int_0^\theta y g_{(n)}(y) dy = ?$

$y \in (0, \theta)$:

$F_Y(y) = \int_0^y f_Y(u) du$

$= \int_0^y \frac{\alpha u^{\alpha-1}}{\theta^\alpha} du$

$= \frac{\alpha}{\theta^\alpha} \int_0^y u^{\alpha-1} du$

$= \frac{\alpha}{\theta^\alpha} \cdot \frac{y^\alpha}{\alpha} = \left(\frac{y}{\theta}\right)^\alpha$

$E[Y_{(n)}] = \int_0^\theta y \cdot n \cdot \left(\frac{y}{\theta}\right)^{\alpha(n-1)} \cdot \frac{\alpha y^{\alpha-1}}{\theta^\alpha} dy$

$= n \cdot \alpha \cdot \frac{1}{\theta^{n\alpha}} \int_0^\theta y \cdot y^{\alpha(n-1)} \cdot y^{\alpha-1} dy$

$= \frac{n\alpha}{\theta^{n\alpha}} \cdot \int_0^\theta y^{n\alpha} dy = \frac{n\alpha}{\theta^{n\alpha}} \cdot \frac{\theta^{n\alpha+1}}{n\alpha+1} = \frac{n\alpha}{n\alpha+1} \cdot \theta$

Not unbiased!

Let's define:

$$\hat{\Theta}' = \frac{n\alpha+1}{n\alpha} \cdot \hat{\Theta} = \frac{n\alpha+1}{n\alpha} \cdot Y_{(n)}$$

unbiased 😊

$$\text{MSE}[\hat{\Theta}] = \text{Var}[\hat{\Theta}] + \underbrace{(\text{bias}(\hat{\Theta}))^2}_{=0} = \text{Var}[\hat{\Theta}']$$

$$= \text{Var}\left[\frac{n\alpha+1}{n\alpha} \cdot Y_{(n)}\right] = \left(\frac{n\alpha+1}{n\alpha}\right)^2 \text{Var}[Y_{(n)}]$$

$$\text{Var}[Y_{(n)}] = \mathbb{E}[Y_{(n)}^2] - (\mathbb{E}[Y_{(n)}])^2$$

$$\begin{aligned} \int_0^{\Theta} y^2 \cdot g_{(n)}(y) dy &= \int_0^{\Theta} y^2 \cdot n \cdot \frac{\alpha y^{\alpha-1}}{\Theta^{\alpha}} \cdot \left(\left(\frac{y}{\Theta}\right)^{\alpha}\right)^{n-1} dy \\ &= \frac{n\alpha}{\Theta^{n\alpha}} \int_0^{\Theta} y^{\alpha n+1} dy = \frac{n\alpha}{\Theta^{n\alpha}} \cdot \frac{\Theta^{n\alpha+2}}{n\alpha+2} = \frac{n\alpha}{n\alpha+2} \cdot \Theta^2 \end{aligned}$$

$$\text{Var}[Y_{(n)}] = \frac{n\alpha}{n\alpha+2} \Theta^2 - \left(\frac{n\alpha}{n\alpha+1}\right)^2 \cdot \Theta^2$$

$$\text{MSE}[\hat{\Theta}'] = \frac{(n\alpha+1)^2}{(n\alpha)^2} \left(\frac{n\alpha}{n\alpha+2} - \frac{(n\alpha)^2}{(n\alpha+1)^2} \right) \Theta^2$$

$$= \left(\frac{(n\alpha+1)^2}{n\alpha(n\alpha+2)} - 1 \right) \Theta^2$$

$$= \frac{(n\alpha+1)^2 - n\alpha(n\alpha+2)}{n\alpha(n\alpha+2)} \cdot \Theta^2$$

$$= \frac{\cancel{(n\alpha)^2} + 2n\alpha + 1 - \cancel{(n\alpha)^2} - 2n\alpha}{n\alpha(n\alpha+2)} \theta^2$$

$$= \frac{1}{n\alpha(n\alpha+2)} \cdot \theta^2$$

